uniana/tcfg/TcfgEdge.v
@@ -276,4 +276,111 @@ Section cfg.
     all:exfalso;edge_excl.
   Qed.
 
+  Lemma tag_exit_eq' h p q i j
+        (Hedge : (p,i) -t> (q,j))
+        (Hexit : exit_edge h p q)
+    : exists n, i = n :: j.
+  Proof.
+    destruct Hedge.
+    unfold eff_tag in H0.
+    decide (edge__P p q);[|congruence].
+    destruct (edge_Edge e);try edge_excl.
+    destruct i.
+    - exfalso.
+      congruence.
+    - inv H0. eexists; reflexivity.
+  Qed.
+
+  Lemma tcfg_edge_edge (q p : Lab) (i j : Tag)
+        (Hedge : (q,j) -t> (p,i))
+    : edge__P q p.
+  Proof.
+    destruct Hedge. auto.
+  Qed.
+
+  Lemma no_entry_STag (i j : Tag)
+    : 0 :: i <> STag j.
+  Proof.
+    destruct j;cbn;congruence.
+  Qed.
+
+  Lemma tcfg_edge_eq_loop q1 q2 j p i
+        (Hedge1 : (q1,j) -t> (p,i))
+        (Hedge2 : (q2,j) -t> (p,i))
+    : eq_loop q1 q2.
+  Proof.
+    copy Hedge1 Htedge1.
+    copy Hedge2 Htedge2.
+    eapply tcfg_edge_destruct' in Hedge1.
+    eapply tcfg_edge_destruct' in Hedge2.
+    destruct Hedge1 as [Hedge1|[Hedge1|[Hedge1|Hedge1]]].
+    all: destruct Hedge2 as [Hedge2|[Hedge2|[Hedge2|Hedge2]]].
+    all: destruct Hedge1 as [Htag1 Hedge1].
+    all: destruct Hedge2 as [Htag2 Hedge2].
+    all: repeat
+            lazymatch goal with
+            | H : basic_edge _ _ |- _ => eapply basic_edge_eq_loop in H
+            | H : back_edge _ _ |- _ => eapply back_edge_eq_loop in H
+            end.
+    all: lazymatch goal with
+         | H : eq_loop _ _, Q : eq_loop _ _ |- _ => try (rewrite Hedge1,Hedge2;eauto;try reflexivity)
+         | _ => idtac
+         end.
+    all: subst i.
+    all: unfold eexit_edge in *; repeat destructH.
+    all: try lazymatch goal with
+             | H: exit_edge _ _ _ |- _ => eapply tag_exit_eq' in H as Hexit;eauto;destructH
+             end.
+    all: lazymatch goal with
+         | H : _ :: ?x = ?x |- _
+           => eapply list_cycle in H;contradiction
+         | H : ?x = _ :: ?x |- _
+           => symmetry in H; eapply list_cycle in H;contradiction
+         | _ => idtac
+         end.
+    all: lazymatch goal with
+         | H : 0 :: _ = STag _ |- _
+           => eapply no_entry_STag in H;contradiction
+         | H : STag _ = 0 :: _ |- _
+           => symmetry in H; eapply no_entry_STag in H;contradiction
+         | _ => idtac
+         end.
+    all: lazymatch goal with
+         | H : eq_loop _ _, Q : exit_edge _ _ _ |- _
+           => eapply exit_not_deq in Q;
+               [contradiction|eapply exit_pred_loop in Q;
+                              [eapply loop_contains_deq_loop in Q;eapply eq_loop1;eauto
+                              |eapply tcfg_edge_edge;eauto]]
+         | _ => idtac
+         end.
+    2: exfalso;eapply list_cycle2;cbn in *;eauto.
+    2: exfalso;destruct j;cbn in *;[congruence|eapply list_cycle2;symmetry;eauto].
+    - eapply deq_loop_entry in Hedge1 as Hentry1.
+      eapply deq_loop_entry in Hedge2 as Hentry2.
+      split.
+      + intros h Hh.
+        decide (h = p).
+        * exfalso. subst. destruct Hedge2. destruct H0. contradiction.
+        * eapply deq_loop_entry_or in Hedge1. 2:eauto. destruct Hedge1;[assumption|contradiction].
+      + intros h Hh.
+        decide (h = p).
+        * exfalso. subst. destruct Hedge1. destruct H0. contradiction.
+        * eapply deq_loop_entry_or in Hedge2. 2:eauto. destruct Hedge2;[assumption|contradiction].
+    - eapply deq_loop_exiting in Hedge1 as Hdeq1.
+      eapply deq_loop_exiting in Hedge2 as Hdeq2.
+      eapply exit_pred_loop in Hedge1. 2: eapply tcfg_edge_edge in Htedge2;eauto.
+      eapply exit_pred_loop in Hedge2. 2: eapply tcfg_edge_edge in Htedge1;eauto.
+      eapply loop_contains_deq_loop in Hedge1.
+      eapply loop_contains_deq_loop in Hedge2.
+      split;[transitivity h|transitivity h0];eauto.
+  Qed.
+
+
+  Lemma nexit_injective q1 q2 p1 p2 j1 j2 i
+        (Hedge1 : (q1,j1) -t> (p1,i))
+        (Hedge2 : (q2,j2) -t> (p2,i))
+        (Hnexit1 : nexit_edge q1 p1)
+    : j1 = j2.
+  Admitted.
+
 End cfg.
